cedar-lean/Cedar/Thm/Translation.lean
@@ -1,0 +1,17 @@
+import Cedar.Spec
+import Cedar.Spec.Cst
+import Cedar.Spec.CstSemantics
+import Cedar.Spec.CstToAst
+
+namespace Cedar.Thm
+
+open Cedar.Data
+open Cedar.Spec
+
+-- First show that the decision is the same
+-- Then match policyIDs
+
+theorem translation_is_sound (cps : Cst.Policies) (aps : Spec.Policies)
+(req : Request) (es : Entities) :
+  cps.toPolicies? = some aps →
+  Cst.isAuthorized req es cps = Spec.isAuthorized req es aps := sorry
