cedar-lean/Cedar/Thm/Translation/ExprTranslation.lean
@@ -1,0 +1,66 @@
+import Cedar.Spec
+import Cedar.Spec.Cst
+import Cedar.Spec.CstSemantics
+import Cedar.Spec.CstToAst
+
+namespace Cedar.Thm
+
+open Cedar.Data
+open Cedar.Spec
+
+mutual
+
+theorem exprOrSpecial_to_expr_evalute (eos : ExprOrSpecial) (aexp : Expr)
+  (req : Request) (es : Entities) :
+  eos.toExpr? = some aexp →
+  evaluate aexp req es = match eos with
+  | .expr e => evaluate e req es
+  | .var v => evaluate (Expr.var v) req es
+  | .strLit s => (CstCommon.unescape? s).elim
+            (.error .typeError)
+            (fun s' => .ok (.prim (.string s')))
+  | .boolLit b => .ok (.prim (.bool b))
+  | .name _ => .error .typeError := by
+  cases eos <;> intro h <;> simp_all [ExprOrSpecial.toExpr?]
+  · rename_i lit; cases hsome : CstCommon.unescape? lit with
+    | none => rw [hsome] at h; simp at h
+    | some s' => rw [hsome] at h; simp at *; rw [← h]; simp [evaluate]
+  · rename_i b; rw [← h]; simp [evaluate]
+
+theorem primary_to_expr_evaluate
+  (prim : Cst.Primary) (eos : ExprOrSpecial)
+  (req : Request) (es : Entities) :
+  prim.toExprOrSpecial? = some eos →
+  ∀ aexp, eos.toExpr? = some aexp →
+  evaluate aexp req es = prim.evaluate req es := by
+  cases prim
+  · /- .literal -/
+    intro hprim aexp heos; rename_i lit
+    simp [Cst.Primary.toExprOrSpecial?, Cst.Literal.toExprOrSpecial?] at hprim
+    have haexp := exprOrSpecial_to_expr_evalute eos aexp req es heos
+    rw [haexp]; clear haexp
+    cases lit <;> simp at hprim <;> try rw [← hprim]
+    · /- .liTrue -/
+      unfold Cst.Primary.evaluate; simp
+    · /- .liFalse -/
+      unfold Cst.Primary.evaluate; simp
+    · /- .liNum -/
+      rename_i n; unfold Cst.Primary.evaluate; simp; cases hn: (Int64.ofInt? ↑n.toNat) with
+      | none => rw [hn] at hprim; simp at *
+      | some n' => rw [hn] at hprim; simp at *; rw [← hprim]; simp; simp [evaluate]
+    · /- .liStr -/
+      rename_i s; unfold Cst.Primary.evaluate; simp; cases hs: (CstCommon.unescape? s) <;> simp
+
+  sorry
+
+
+
+
+
+
+theorem expr_translation_sound (cexp : Cst.Expr) (aexp : Expr) (req : Request) (es : Entities) :
+  cexp.toAExpr? = some aexp →
+  cexp.evaluate req es = evaluate aexp req es := by sorry
+
+
+end
